refactor(Testing): remove callbacks + support for compact semantics

coq/Testing.v
@@ -1,173 +1,195 @@
 Require Import Koika.Frontend.
 Require Import Coq.Program.Equality.
+Require Koika.CompactLogs
+        Koika.CompactSemantics.
+
+Module CL := Koika.CompactLogs.
+Module CS := Koika.CompactSemantics.
 
 (* This dependently-typed function is required for the type of the context. *)
 Definition input { sig : list (string * type) } := context ( fun (x : (string * type)) => type_denote (snd x) ) sig.
+Notation "'assert' a ':=' b 'in' body" := (match b with | a => body | _ => False end) (at level 200, a pattern).
 
-(**
- * # run_function'
- *
- * This function can be used to compute a koika function.
- * 
- * Note: It could also be used for actions, but we also provide
- *       [run_action'] to implicitly pass no function arguments.
- *
- * # Arguments
- * 
- * - r            : register value assignment
- * - sigma_denote : coq implementations of external functions
- * - inputs       : direct inputs to the function
- * - func         : the actual koika function to run
- * - callback     : a callback function that is run on the
- *                  function's result if it didn't fail
- *
- * # Callback Arguments
- *
- * - ctxt : a koika context, holding the new register values
- * - out  : the direct output of the function
- *
- * # Examples
- *
- * see []()
- *)
-Definition run_function'
-  { reg_t : Type }
- `{ FiniteType reg_t }
-  { sig : tsig var_t }
-  { tau }
-  { ext_fn_t : Type }
-  { sigma : (ext_fn_t -> ExternalSignature) }
-  { R : reg_t -> type }
-  ( r : (forall reg : reg_t, R reg) )
-  ( sigma_denote : (forall fn: ext_fn_t, Sig_denote (sigma fn)) )
-  ( inputs : input )
-  ( func : action R sigma sig tau )
-  ( callback : env_t ContextEnv R -> tau -> Prop )
-  : Prop :=
-    let env := ContextEnv.(create) r in
-    match (* tc_compute? *) (interp_action env sigma_denote inputs log_empty log_empty func) with
-    | Some (log,out,_) =>
-      let ctxt := commit_update env log in
-      callback ctxt out
-    | None => False
-    end.
+Section EvaluationUtilities.
+  Context  [reg_t : Type ].
+  Context `[FiniteType reg_t].
+  Context  [R : reg_t -> type].
+  Context  (r : (forall reg : reg_t, R reg)).
+  Context  {tau : type}.
 
-(**
- * # run_action
- *
- * Utility function of [run_function']
- *
- * In contrast to [run_function'] this function does not expect a function input
- * this might be handy to test actions instead of functions.
- * Additionally, the callback does not provide an output, only a context.
- *
- * # Arguments
- *
- * see [run_function']
- *)
-Definition run_action'
-  { reg_t }
- `{ FiniteType reg_t }
-  { tau }
-  { ext_fn_t }
-  { sigma }
-  { R : reg_t -> type }
-  ( r : (forall reg : reg_t, R reg) )
-  ( sigma_denote : (forall fn: ext_fn_t, Sig_denote (sigma fn)) )
-  ( func : action R sigma [] tau )
-  ( callback : env_t ContextEnv R -> Prop )
-  : Prop :=
-    run_function' r sigma_denote CtxEmpty func (fun ctxt out => callback ctxt).
+  Section Sigma.
 
+    Context [ ext_fn_t : Type ].
+    Context [ sigma : (ext_fn_t -> ExternalSignature) ].
+    Context ( sigma_denote : (forall fn: ext_fn_t, Sig_denote (sigma fn)) ).
 
-(**
- * # run_function
- *
- * Utility function of [run_function']
- *
- * In contrast to [run_function'] this expects an empty external function
- * signature.
- *
- * # Arguments
- *
- * see [run_function']
- *)
-Definition run_function
-  { reg_t : Type }
- `{ FiniteType reg_t }
-  { tau }
-  { sig : tsig var_t }
-  { R : reg_t -> type }
-  ( r : (forall reg : reg_t, R reg) )
-  ( inputs : input )
-  ( func : action R empty_Sigma sig tau )
-  ( callback : env_t ContextEnv R -> tau -> Prop )
-  : Prop :=
-    run_function' r empty_sigma inputs func callback.
+    (**
+     * # run_function'
+     *
+     * This function can be used to compute a koika function.
+     *
+     * Note: It could also be used for actions, but we also provide
+     *       [run_action'] to implicitly pass no function arguments.
+     *
+     * # Arguments
+     *
+     * - r            : register value assignment
+     * - sigma_denote : coq implementations of external functions
+     * - inputs       : direct inputs to the function
+     * - func         : the actual koika function to run
+     * - callback     : a callback function that is run on the
+     *                  function's result if it didn't fail
+     *
+     * # Callback Arguments
+     *
+     * - ctxt : a koika context, holding the new register values
+     * - out  : the direct output of the function
+     *
+     * # Examples
+     *
+     * see []()
+     *)
+    Definition run_function'
+      [ sig : tsig var_t ]
+      ( inputs : input )
+      ( func : action R sigma sig tau )
+      : option (ContextEnv.(env_t) R * tau) :=
+        let env := ContextEnv.(create) r in
+        option_map (fun '(log,out,_) => (commit_update env log, out))
+          (interp_action env sigma_denote inputs log_empty log_empty func).
 
-(**
- * # run_action
- *
- * Utility function of [run_action']
- *
- * In contrast to [run_action'] this expects an empty external function
- * signature.
- *
- * # Arguments
- *
- * see [run_action']
- *)
-Definition run_action
-  { reg_t }
- `{ FiniteType reg_t }
-  { tau }
-  { R : reg_t -> type }
-  ( r : (forall reg : reg_t, R reg) )
-  ( func : action R empty_Sigma [] tau )
-  ( callback : env_t ContextEnv R -> Prop )
-  : Prop :=
-    run_action' r empty_sigma func callback.
+    (**
+     * # run_funcion_cs'
+     *
+     * This is a compact sematics variant of [run_function']
+     *)
+    Definition run_function_cs'
+      [ sig : tsig var_t ]
+      ( inputs : input )
+      ( func : action R sigma sig tau )
+      : option (ContextEnv.(env_t) R * tau) :=
+        let env := ContextEnv.(create) r in
+        option_map (fun '(log,out,_) => (CL.commit_update env log, out))
+          (CS.interp_action env sigma_denote inputs CL.log_empty CL.log_empty func).
 
-(**
- * # run_schedule
- *
- * This function can be used to compute a koika action or function
- *
- * # Arguments
- *
- * - r            : register value assignment
- * - rules        : mapping of rule names to actions
- * - sigma_denote : implementations of external functions
- * - sched        : the scheduler to run
- * - callback     : this function is invoked on the resulting
- *                  context
- *
- * # Callback Arguments
- *
- * - ctxt     : a koika context, holding new register values
- *
- * # Examples
- *
- * TODO
- *)
-Definition run_schedule
-  { reg_t : Type }
-  { ext_fn_t : Type }
- `{ FiniteType reg_t }
-  { R : reg_t -> type }
-  { rule_name_t : Type }
-  { sigma : (ext_fn_t -> ExternalSignature) }
+    (**
+     * # run_action'
+     *
+     * Utility function of [run_function']
+     *
+     * In contrast to [run_function'] this function does not expect a function input
+     * this might be handy to test actions instead of functions.
+     * Additionally, the callback does not provide an output, only a context.
+     *
+     * # Arguments
+     *
+     * see [run_function']
+     *)
+    Definition run_action' func :=
+        option_map (fun '(ctxt,out) => ctxt)
+          (run_function' CtxEmpty func).
 
-  ( r : (forall reg : reg_t, R reg) )
-  ( rules : rule_name_t -> action R sigma [] unit_t )
-  ( sigma_denote : (forall fn: ext_fn_t, Sig_denote (sigma fn)) )
-  ( sched : scheduler )
-  ( callback : env_t ContextEnv R -> Prop )
+    (**
+     * # run_action_cs'
+     *
+     * This is a compact sematics variant of [run_action']
+     *)
+    Definition run_action_cs' func :=
+        option_map (fun '(ctxt,out) => ctxt)
+          (run_function_cs' CtxEmpty func).
 
-  : Prop :=
-    let env := ContextEnv.(create) r in
-    let log := interp_scheduler env sigma_denote rules sched in
-      callback (commit_update env log).
+    (**
+     * # run_schedule
+     *
+     * This function can be used to compute a koika action or function
+     *
+     * # Arguments
+     *
+     * - r            : register value assignment
+     * - rules        : mapping of rule names to actions
+     * - sigma_denote : implementations of external functions
+     * - sched        : the scheduler to run
+     * - callback     : this function is invoked on the resulting
+     *                  context
+     *
+     * # Callback Arguments
+     *
+     * - ctxt     : a koika context, holding new register values
+     *
+     * # Examples
+     *
+     * TODO
+     *)
+    Definition run_schedule
+      [ rule_name_t ]
+      ( rules : rule_name_t -> action R sigma [] unit_t )
+      ( sched : scheduler )
+      : ContextEnv.(env_t) R :=
+        let env := ContextEnv.(create) r in
+        let log := interp_scheduler env sigma_denote rules sched in
+        (commit_update env log).
+
+    (**
+     * # run_schedule_cs
+     *
+     * This is a compact sematics variant of [run_schedule]
+     *)
+    Definition run_schedule_cs
+      [ rule_name_t ]
+      ( rules : rule_name_t -> action R sigma [] unit_t )
+      ( sched : scheduler )
+      : ContextEnv.(env_t) R :=
+        let env := ContextEnv.(create) r in
+        let log := CS.interp_scheduler env sigma_denote rules sched in
+        (CL.commit_update env log).
+  End Sigma.
+
+  (**
+  * # run_function
+  *
+  * Utility function of [run_function']
+  *
+  * In contrast to [run_function'] this expects an empty external function
+  * signature.
+  *
+  * # Arguments
+  *
+  * see [run_function']
+  *)
+  Definition run_function [sig] :=
+      run_function' empty_sigma (sig := sig).
+
+  (**
+   * # run_function_cs
+   *
+   * This is a compact sematics variant of [run_function]
+   *)
+  Definition run_function_cs [sig] :=
+    run_function_cs' empty_sigma (sig := sig).
+
+  (**
+  * # run_action
+  *
+  * Utility function of [run_action']
+  *
+  * In contrast to [run_action'] this expects an empty external function
+  * signature.
+  *
+  * # Arguments
+  *
+  * see [run_action']
+  *)
+  Definition run_action :=
+      run_action' empty_sigma.
+
+  (**
+   * # run_action_cs
+   *
+   * This is a compact sematics variant of [run_action]
+   *)
+   Definition run_action_cs :=
+    run_action_cs' empty_sigma.
+End EvaluationUtilities.
 
 
 Ltac check :=
